conquord/src/conquord/Ex_Sum.v
@@ -1,0 +1,84 @@
+Require Import conquord.Language conquord.Interpret conquord.Value conquord.TypeSystem conquord.TypeSound
+  conquord.TransfSound conquord.IndexInterface conquord.CollectionTransf conquord.DictIndexImpl
+  conquord.SumAgg conquord.MinAgg conquord.BitmapIndex conquord.TransfUtils conquord.RelTransf conquord.IndexTransf
+  conquord.Utils conquord.Substitute conquord.OptimizeAnno conquord.ToPython.
+Require Import coqutil.Map.Interface coqutil.Map.SortedListString coqutil.Word.Interface coqutil.Datatypes.Result.
+From Stdlib Require Import List String ZArith.
+
+Import ListNotations.
+
+(*
+(* Materialized view and incremental computation of an aggregation *)
+
+let mut orders := orders_tbl in
+
+foreach q in queries do
+    let mut output := "" in
+    if q.type = 0
+    then
+        let total = sum [ o <- !orders, ret o.value ] in
+        output := "Current total value: " ++
+            str(total) ++ "\n"
+    else
+        orders := q.new_order :: !orders;
+        output := "Added a new order\n"
+    end;
+    outputs := !output :: !outputs
+end
+*)
+
+Definition prog := (CLetMut (EVar "orders_tbl") "orders" (CForeach (EVar "queries") "q" (CLetMut (EAtom (AString "")) "output" (CSeq (CIf (EBinop OEq (EAccess (EVar "q") "type") (EAtom (AInt 0))) (CLet (EFold (EFlatmap LikeList (ELoc "orders") "o" (EBinop OCons (EAccess (EVar "o") "value") (EAtom (ANil None)))) (EAtom (AInt 0)) "_v" "_acc" (EBinop OPlus (EVar "_v") (EVar "_acc"))) "total" (CAssign "output" (EBinop OConcatString (EAtom (AString "Current total value: ")) (EBinop OConcatString (EUnop OIntToString (EVar "total")) (EAtom (AString "\n")))))) (CSeq (CAssign "orders" (EBinop OCons (EAccess (EVar "q") "new_order") (ELoc "orders"))) (CAssign "output" (EAtom (AString "Added a new order\n"))))) (CAssign "outputs" (EBinop OCons (ELoc "output") (ELoc "outputs"))))))).
+
+(* Claude Sonnet 4.6 *)
+Definition heuristics :=
+  [ AC [PushdownCollection; AnnotateCollection; ToProj]
+      [[SumAgg "value"]]
+  ].
+
+Definition row_ty_orders :=
+  TRecord (record_sort [("id", TInt); ("value", TInt)]).
+
+Definition row_ty_query :=
+  TRecord (record_sort [("type", TInt); ("new_order", row_ty_orders)]).
+
+Section WithConcreteMaps.
+  Context {width: Z} {word: word.word width} {word_ok: word.ok word}.
+  Notation value := (value (width:=width)).
+
+  Local Open Scope string.
+
+  Instance ctenv : map.map string type := SortedListString.map _.
+  Instance ctenv_ok : map.ok ctenv := SortedListString.ok _.
+
+  Instance clocals : map.map string value := SortedListString.map _.
+  Instance clocals_ok : map.ok clocals := SortedListString.ok _.
+
+  Definition init_Gstore : ctenv :=
+    map.put map.empty "outputs" (TList TString).
+
+  Definition init_Genv : ctenv :=
+    map.put (map.put map.empty "orders_tbl" (TList row_ty_orders))
+      "queries" (TList row_ty_query).
+
+  Compute (typecheck init_Gstore init_Genv prog).
+
+  Definition prog_transformed := map (fun heu => apply_optimize_anno (width:=width) (heu prog) init_Gstore init_Genv) heuristics.
+
+  Compute prog_transformed.
+
+  Theorem prog_transformed_sem : forall (store env : clocals),
+      locals_wf init_Gstore store ->
+      locals_wf init_Genv env ->
+      forall prog', In prog' prog_transformed ->
+                    interp_command store env prog' = interp_command store env prog.
+  Proof.
+    unfold prog_transformed, heuristics, apply_optimize_anno; cbn [map]; intros.
+    repeat destruct_In;
+      try eapply transf_sound__preserve_sem;
+      eauto using apply_all_transfs_sound with transf_hints.
+    lazymatch goal with H: In _ [] |- _ => apply in_nil in H; intuition idtac end.
+  Qed.
+End WithConcreteMaps.
+
+Compute program_py prog.
+Compute map program_py prog_transformed.
