conquord/src/conquord/Interpret.v
@@ -1,4 +1,4 @@
-Require Import ZArith String List DecimalString.
+From Stdlib Require Import ZArith String List DecimalString.
 Require Import conquord.Language conquord.Value.
 Require Import coqutil.Word.Interface coqutil.Map.Interface coqutil.Datatypes.Result.
 
