conquord/src/conquord/OptimizeAnno.v
@@ -1,0 +1,594 @@
+Require Import conquord.Language conquord.Interpret conquord.Value conquord.TypeSystem conquord.TypeSound conquord.IndexInterface
+  conquord.CollectionTransf conquord.DictIndexImpl conquord.SumAgg conquord.MinAgg conquord.BitmapIndex conquord.TransfUtils conquord.RelTransf conquord.IndexTransf conquord.TransfSound conquord.Utils conquord.Substitute.
+Require Import coqutil.Map.Interface coqutil.Map.SortedListString coqutil.Word.Interface coqutil.Datatypes.Result.
+From Stdlib Require Import List String ZArith Permutation.
+Import ListNotations.
+
+Require Import conquord.Notations.
+Open Scope conquord_scope.
+
+Variant basic_transf :=
+  | SwapIfNil
+  | MergeIf
+  | SplitIf
+  | SwapFlatmapIf
+  | IfNilIntoFlatmap
+  | ToFilter
+  | ToProj
+  | ToJoin
+  | SwapConjuncts
+  | JoinToFlatmapFilter
+  | FilterPushdown
+  | AnnotateCollection
+  | PushdownCollection.
+
+Variant index_choice :=
+  | SumAgg (attr : string)
+  | MinAgg (attr : string)
+  | DictIdx (attr : string)
+  | BitmapIdx (attr : string) (attr_v : string).
+
+Variant anno_command :=
+  | AC (basic_transfs : list basic_transf) (all_index_choices : list (list index_choice)) (c : command).
+
+Definition to_proj_transf := fold_command id to_proj_head.
+Definition to_filter_transf := fold_command id to_filter_head.
+Definition to_join_transf := fold_command id to_join_head.
+Definition annotate_collection_transf := fold_command id annotate_collection.
+Definition push_down_collection_transf := fold_command id push_down_collection.
+Definition filter_pushdown_transf := fold_command id filter_pushdown_head.
+Definition swap_if_nil_transf := fold_command id swap_if_nil_head.
+Definition merge_if_transf := fold_command id merge_if_head.
+Definition split_if_transf := fold_command id split_if_head.
+Definition swap_flatmap_if_transf := fold_command id swap_flatmap_if_head.
+Definition if_nil_into_flatmap_transf := fold_command id if_nil_into_flatmap_head.
+Definition join_to_flatmap_filter_transf := fold_command id join_to_flatmap_filter_head.
+Definition swap_conjuncts_transf := fold_command id swap_conjuncts_head.
+
+Definition mk_basic_transf (f : basic_transf) : command -> command :=
+  match f with
+  | SwapIfNil => swap_if_nil_transf
+  | MergeIf => merge_if_transf
+  | SplitIf => split_if_transf
+  | SwapFlatmapIf => swap_flatmap_if_transf
+  | IfNilIntoFlatmap => if_nil_into_flatmap_transf
+  | ToFilter => to_filter_transf
+  | ToProj => to_proj_transf
+  | ToJoin => to_join_transf
+  | SwapConjuncts => swap_conjuncts_transf
+  | JoinToFlatmapFilter => join_to_flatmap_filter_transf
+  | FilterPushdown => filter_pushdown_transf
+  | AnnotateCollection => annotate_collection_transf
+  | PushdownCollection => push_down_collection_transf
+  end.
+
+Definition compose_basic_transfs : list (command -> command) -> command -> command :=
+  fold_right Basics.compose id.
+
+Section WithConcreteMaps.
+  Context {width: Z} {word: word.word width} {word_ok: word.ok word}.
+  Notation value := (value (width:=width)).
+
+  Local Open Scope string.
+
+  Instance ctenv : map.map string type := SortedListString.map _.
+  Instance ctenv_ok : map.ok ctenv := SortedListString.ok _.
+
+  Instance clocals : map.map string value := SortedListString.map _.
+  Instance clocals_ok : map.ok clocals := SortedListString.ok _.
+
+  Section CommonPipelineParts.
+    Context (tag tag' : string).
+    Context (sum_agg_attr : string).
+
+    Definition sum_agg_wf := (SumAgg.idx_wf (locals:=clocals) "hole" sum_agg_attr "x").
+    Instance csum_agg : IndexInterface.index := (sum_agg "hole" sum_agg_attr "x").
+    Instance csum_agg_ok : IndexInterface.ok csum_agg sum_agg_wf.
+    apply sum_agg_ok.
+    Qed.
+
+    Definition sum_agg_lookup_transf := fun tbl => fold_command_with_globals [tbl] (sum_to_agg_lookup_head sum_agg_attr "id_tag" "aux_tag" tag tbl).
+    Definition cons_to_add_transf := fun tbl => fold_command_with_globals [tbl] (cons_to_add_head).
+
+    Context (min_agg_attr : string).
+
+    Definition min_agg_wf := (MinAgg.idx_wf (locals:=clocals) "hole" min_agg_attr "x").
+    Instance cmin_agg : IndexInterface.index := (min_agg "hole" min_agg_attr "x").
+    Instance cmin_agg_ok : IndexInterface.ok cmin_agg min_agg_wf.
+    apply min_agg_ok.
+    Qed.
+
+    Definition min_agg_lookup_transf := fun tbl => fold_command_with_globals [tbl] (min_to_agg_lookup_head min_agg_attr "id_tag" "aux_tag" tag tbl).
+    Definition cons_to_min_transf := fun tbl => fold_command_with_globals [tbl] (cons_to_min_head "y").
+
+    Context (dict_idx_attr : string).
+
+    Definition dict_idx_wf := (DictIndexImpl.idx_wf (width:=width) "hole" dict_idx_attr "tup" "acc" "x").
+    Instance cdict_idx : IndexInterface.index := (dict_idx "hole" dict_idx_attr "tup" "acc" "x").
+    Instance cdict_idx_ok : IndexInterface.ok cdict_idx dict_idx_wf.
+    apply dict_idx_ok. auto with transf_hints.
+    Qed.
+
+    Definition dict_lookup_transf := fun tbl => fold_command_with_globals [tbl] (eq_filter_to_lookup_head dict_idx_attr "id_tag" "aux_tag" tag "b" tbl).
+    Definition cons_to_insert_transf := fun tbl => fold_command_with_globals [tbl] (cons_to_insert_head dict_idx_attr "tup" "acc" "x" "y").
+    Definition use_dict_idx_transf := fun tbl => fold_command_with_globals [tbl] (use_idx_head dict_idx_attr "id_tag" "aux_tag" tag tbl).
+
+    Definition pk_idx_wf := (BitmapIndex.pk_idx_wf (width:=width) "hole" "tup" "acc").
+    Instance cpk_idx : IndexInterface.index := (pk_idx "hole" "tup" "acc").
+    Instance cpk_idx_ok : IndexInterface.ok cpk_idx pk_idx_wf.
+    apply pk_idx_ok. auto with transf_hints.
+    Qed.
+
+    Context (bitmap_attr : string).
+    Context (bitmap_str : string).
+    Definition bitmap_wf := (bitmap_wf (width:=width) bitmap_attr bitmap_str "hole" "tup").
+    Instance bitmap : IndexInterface.index := (bitmap bitmap_attr bitmap_str "hole" "tup").
+    Instance bitmap_ok : IndexInterface.ok bitmap bitmap_wf.
+    apply bitmap_ok.
+    Qed.
+
+    Definition cons_to_pk_idx_update_transf := fun tbl => fold_command_with_globals [tbl] (cons_to_pk_idx_update_head "y").
+    Definition use_pk_idx_transf := fun tbl => fold_command_with_globals [tbl] (use_pk_idx_head "id_tag" "aux_tag" tag tbl).
+    Definition cons_to_bitmap_update_transf := fun tbl => fold_command_with_globals [tbl] cons_to_bitmap_update_head.
+    Definition use_bitmap_transf := fun tbl => fold_command_with_globals [tbl] (use_bitmap_head bitmap_attr bitmap_str "id_tag" "aux_tag" tag tbl).
+    Definition filter_to_bitmap_lookup_transf :=
+      fun tbl => fold_command_with_globals [tbl]
+                   (filter_to_bitmap_lookup_head bitmap_attr bitmap_str "id_tag" "aux_tag" tag tag' "x" "b" "acc" tbl).
+  End CommonPipelineParts.
+
+  Definition mk_idx (cur_tag : nat) (reps : nat) (ic : index_choice) :
+    list (string * IndexInterface.index * (value -> value -> Prop)) * list (string -> command -> command) * nat :=
+    match ic with
+    | SumAgg attr =>
+        let sum_tag := String.of_nat cur_tag in
+        ([(sum_tag, csum_agg attr, sum_agg_wf attr)],
+          [sum_agg_lookup_transf sum_tag attr;
+           fun tbl => repeat_transf (cons_to_add_transf tbl) reps],
+          S cur_tag)
+    | MinAgg attr =>
+        let min_tag := String.of_nat cur_tag in
+        ([(min_tag, cmin_agg attr, min_agg_wf attr)],
+                       [min_agg_lookup_transf min_tag attr;
+                        fun tbl => repeat_transf (cons_to_min_transf tbl) reps],
+          S cur_tag)
+    | DictIdx attr =>
+        let dict_idx_tag := String.of_nat cur_tag in
+        ([(dict_idx_tag, cdict_idx attr, dict_idx_wf attr)],
+          [dict_lookup_transf dict_idx_tag attr;
+           use_dict_idx_transf dict_idx_tag attr;
+           fun tbl => repeat_transf (cons_to_insert_transf attr tbl) reps],
+          S cur_tag)
+    | BitmapIdx attr v =>
+        let pk_idx_tag := String.of_nat cur_tag in
+        let bm_tag := String.of_nat (S cur_tag) in
+        ([(pk_idx_tag, cpk_idx, pk_idx_wf);
+          (bm_tag, bitmap attr v, bitmap_wf attr v)],
+          [filter_to_bitmap_lookup_transf pk_idx_tag bm_tag attr v;
+           use_bitmap_transf bm_tag attr v;
+           fun tbl => repeat_transf (cons_to_bitmap_update_transf tbl) reps;
+           use_pk_idx_transf pk_idx_tag;
+           fun tbl => repeat_transf (cons_to_pk_idx_update_transf tbl) reps],
+          S (S cur_tag))
+end.
+
+  Fixpoint mk_idxs (cur_tag : nat) (reps : nat) (ics : list index_choice) :
+    list (string * IndexInterface.index * (value -> value -> Prop)) * list (string -> command -> command) * nat :=
+    match ics with
+    | [] => ([], [], cur_tag)
+    | ic :: ics =>
+        let '(idxs1, transfs1, cur_tag1) := mk_idx cur_tag reps ic in
+        let '(idxs2, transfs2, cur_tag2) := mk_idxs cur_tag1 reps ics in
+        (app idxs1 idxs2, app transfs1 transfs2, cur_tag2)
+    end.
+
+  Definition mk_compo_idx (idxs : list (string * IndexInterface.index * (value -> value -> Prop))) : IndexInterface.index :=
+    compo_idx idxs "hole" (word:=word).
+
+  Lemma Forall_tag_bound_trans : forall a b c l,
+      Forall (fun s => exists n, s = String.of_nat n /\ a <= n < b) l ->
+      c <= a ->
+      Forall (fun s => exists n, s = String.of_nat n /\ c <= n < b) l.
+  Proof.
+    induction l; constructor; invert_Forall; auto.
+    destruct_exists.
+    eexists; intuition eauto using Nat.le_trans.
+  Qed.
+
+  Lemma Forall_tag_bound_trans2 : forall a b c l,
+      Forall (fun s => exists n, s = String.of_nat n /\ a <= n < b) l ->
+      b <= c ->
+      Forall (fun s => exists n, s = String.of_nat n /\ a <= n < c) l.
+  Proof.
+    induction l; constructor; invert_Forall; auto.
+    destruct_exists.
+    eexists; intuition eauto using Nat.le_trans.
+  Qed.
+
+  Lemma mk_idx_ok : forall ic init_tag reps idxs transfs next_tag,
+      (idxs, transfs, next_tag) = mk_idx init_tag reps ic ->
+      init_tag < next_tag /\
+      Forall (fun '(_, idx, idx_wf) => IndexInterface.ok idx idx_wf) idxs /\
+        Forall (fun tag => exists n, tag = String.of_nat n /\ init_tag <= n /\ n < next_tag) (map fst (map fst idxs)) /\
+        NoDup (map fst (map fst idxs)) /\
+        Forall (fun '(_, idx, _) => hole = "hole") idxs.
+  Proof.
+    destruct ic; unfold mk_idx; intros;
+      invert_pair; intuition idtac; constructor; auto using NoDup_nil, csum_agg_ok, cmin_agg_ok, cdict_idx_ok, cpk_idx_ok, bitmap_ok; auto.
+    1-4: eexists; intuition eauto.
+    1:{ repeat constructor. unfold String.of_nat.
+        exists (S init_tag); intuition auto. }
+    1:{ intuition idtac.
+        cbn [fst] in *. destruct_In; auto.
+        apply String.of_nat_inj, Nat.neq_succ_diag_l in H.
+        intuition fail. }
+    1:{ cbn [fst].
+        constructor; auto using NoDup_nil. }
+  Qed.
+
+  Lemma mk_idxs_ok : forall ics init_tag reps idxs transfs next_tag,
+      (idxs, transfs, next_tag) = mk_idxs init_tag reps ics ->
+      init_tag <= next_tag /\
+      Forall (fun '(_, idx, idx_wf) => IndexInterface.ok idx idx_wf) idxs /\
+        Forall (fun tag => exists n, tag = String.of_nat n /\ init_tag <= n /\ n < next_tag) (map fst (map fst idxs)) /\
+        NoDup (map fst (map fst idxs)) /\
+        Forall (fun '(_, idx, _) => hole = "hole") idxs.
+  Proof.
+    induction ics; cbn; intros.
+    1:{ invert_pair; intuition auto using NoDup_nil. }
+    1:{ repeat destruct_match_hyp. invert_pair.
+        intuition idtac.
+        all: lazymatch goal with
+               E: mk_idx _ _ _ = _ |- _ =>
+                 symmetry in E; apply mk_idx_ok in E
+             end; intuition idtac.
+        all: lazymatch goal with
+               E: mk_idxs _ _ _ = _ |- _ =>
+                 symmetry in E; apply IHics in E
+             end; intuition idtac.
+        1:{ eauto using Nat.lt_le_trans, Nat.lt_le_incl. }
+        1:{ apply Forall_app; intuition idtac. }
+        1:{ rewrite !map_app. apply Forall_app; intuition idtac.
+            2: eapply Forall_tag_bound_trans; eauto using Nat.lt_le_trans, Nat.lt_le_incl.
+            eapply Forall_tag_bound_trans2; eauto. }
+        1:{ rewrite !map_app. apply NoDup_app; auto.
+            intros. intro contra. repeat apply_Forall_In.
+            repeat destruct_exists; intuition subst.
+            lazymatch goal with
+              E: String.of_nat _ = String.of_nat _ |- _ =>
+                apply String.of_nat_inj in E
+            end. subst.
+            lazymatch goal with
+              H: ?x <= ?y, _: ?y < ?x |- _ =>
+                apply Nat.le_ngt in H
+            end; intuition idtac. }
+        1:{ apply Forall_app; intuition idtac. } }
+  Qed.
+
+  Lemma mk_compo_idx_ok : forall init_tag reps index_choices idxs transfs next_tag,
+      (idxs, transfs, next_tag) = mk_idxs init_tag reps index_choices ->
+      IndexInterface.ok (mk_compo_idx idxs) (compo_idx_wf idxs).
+  Proof.
+    intros. apply mk_idxs_ok in H; intuition idtac.
+    apply compo_idx_ok; auto.
+  Qed.
+
+  Definition mk_idx_use_transfs (l : list (string -> command -> command)) : string -> command -> command :=
+    fun tbl => fold_right (fun f g => Basics.compose (f tbl) g) id l.
+
+  Definition mk_idx_related_transfs (idx : IndexInterface.index) (f : string -> command -> command) :
+    ctenv -> ctenv -> command -> command :=
+    apply_idx_related_transfs (idx:=idx) "id_tag" "aux_tag" f.
+
+  Fixpoint apply_below_n_letmuts (n : nat) (f : ctenv -> ctenv -> command -> command) :
+    ctenv -> ctenv -> command -> command :=
+    match n with
+    | O => f
+    | S n => apply_below_n_letmuts n (apply_below_letmut f)
+    end.
+
+  Fixpoint compose_all_idx_transfs (n : nat) (l : list (ctenv -> ctenv -> command -> command)) :
+    ctenv -> ctenv -> command -> command :=
+    match l with
+    | [] => fun _ _ => id
+    | f :: l =>
+        fun Gstore Genv =>
+          Basics.compose (apply_below_n_letmuts n f Gstore Genv) (compose_all_idx_transfs (S n) l Gstore Genv)
+    end.
+
+  Definition apply_all_transfs (reps : nat) (fs : list basic_transf) (icss : list (list index_choice)) (Gstore Genv : ctenv) :=
+    let idx_transfs :=
+      map (fun ics =>
+             let '(idxs, transfs, _) := mk_idxs O reps ics in
+             let cidx := mk_compo_idx idxs in
+             let idx_use_transfs := mk_idx_use_transfs transfs in
+             mk_idx_related_transfs cidx idx_use_transfs) icss in
+    (Basics.compose (compose_all_idx_transfs O idx_transfs Gstore Genv) (compose_basic_transfs (map mk_basic_transf fs))).
+
+  Definition apply_optimize_anno (ac : anno_command) (Gstore Genv : ctenv) :=
+    match ac with
+    | AC fs icss c =>
+        apply_all_transfs 10000 fs icss Gstore Genv c
+    end.
+
+  Lemma id_transf_sound : transf_sound (locals:=clocals) (fun _ _ => id).
+  Proof.
+    unfold transf_sound; intuition auto.
+  Qed.
+
+  Hint Resolve id_transf_sound : transf_hints.
+
+  Lemma compose_basic_transfs_sound : forall fs,
+      transf_sound (locals := clocals)
+        (fun _ _ : ctenv =>
+           compose_basic_transfs (map mk_basic_transf fs)).
+  Proof.
+    induction fs; cbn; auto with transf_hints.
+    apply_transf_sound_lemmas; auto.
+    destruct a; eauto with transf_hints.
+  Qed.
+
+  Lemma apply_below_n_letmuts_sound : forall n f,
+      transf_sound (locals:=clocals) f ->
+      transf_sound (locals:=clocals) (apply_below_n_letmuts n f).
+  Proof.
+    induction n; cbn; auto; intros.
+    apply IHn. apply_transf_sound_lemmas.
+    assumption.
+  Qed.
+
+  Lemma compose_all_idx_transfs_sound : forall l n,
+      Forall (transf_sound (locals:=clocals)) l ->
+      transf_sound (locals:=clocals) (compose_all_idx_transfs n l).
+  Proof.
+    induction l; cbn; intros; auto with transf_hints.
+    apply_transf_sound_lemmas; invert_Forall; auto.
+    apply apply_below_n_letmuts_sound.
+    assumption.
+  Qed.
+
+  Lemma id_aug_transf_sound : forall is_tbl_ty aux_ty (aux_wf : value -> Prop),
+      aug_transf_sound is_tbl_ty aux_ty aux_wf (fun _ => id).
+  Proof.
+    unfold aug_transf_sound; cbn; auto.
+  Qed.
+
+  Lemma aug_transf_sound_fold_compose : forall is_tbl_ty aux_ty aux_wf transfs,
+      Forall (aug_transf_sound (locals:=clocals) is_tbl_ty aux_ty aux_wf) transfs ->
+    aug_transf_sound is_tbl_ty aux_ty aux_wf
+    (fun tbl : string =>
+       fold_right
+         (fun f g => Basics.compose (f tbl) g)
+         id transfs).
+  Proof.
+    induction transfs; cbn; intros.
+    1: apply id_aug_transf_sound.
+    invert_Forall.
+    apply_transf_sound_lemmas; auto.
+  Qed.
+
+  Ltac apply_in_nil :=
+    lazymatch goal with
+      H: In _ [] |- _ =>
+        apply in_nil in H; intuition fail
+    end.
+
+  Ltac apply_incl_cons_inv :=
+    lazymatch goal with
+      H: incl (_ :: _) _ |- _ =>
+        apply incl_cons_inv in H; intuition idtac
+    end.
+
+  Lemma map_fst_map_fst : forall A B C D (l : list (A * B * C)) (f : B -> D),
+      map fst (map (fun '(a, b, _) => (a, f b)) l) = map fst (map fst l).
+  Proof.
+    induction l; cbn; auto; intros.
+    repeat case_match; cbn; f_equal.
+    auto.
+  Qed.
+
+  Ltac apply_in_map :=
+    lazymatch goal with
+      H: In _ ?l |- In _ (map ?g ?l) =>
+        apply in_map with (f:=g) in H
+    end.
+
+  Ltac apply_in_map_with_tag :=
+    lazymatch goal with
+      H: In (?tag, _, _) ?l |- In (?tag, _) (map ?g ?l) =>
+        apply in_map with (f:=g) in H
+    end.
+
+  Ltac prove_aux_ty_for_idx :=
+    lazymatch goal with
+      |- aux_ty_for_idx _ _ _ _ _ =>
+        unfold aux_ty_for_idx;
+        intros; cbn; intuition idtac;
+        erewrite NoDup_Permutation_access_record;
+        try apply Permutation.Permutation_sym, Permuted_record_sort
+    end.
+
+  Ltac prove_access_record_idx_ty :=
+    apply NoDup_In_access_record;
+    [ rewrite map_fst_map_fst; assumption
+    | apply_in_map_with_tag; auto ].
+
+  Ltac prove_NoDup_map_fst_sort_map :=
+    eapply Permutation_NoDup; try eassumption;
+    eapply perm_trans;
+    [ | eapply Permutation_map, Permuted_record_sort ];
+    rewrite map_fst_map_fst; auto.
+
+  Ltac prove_In_map_fst_sort_map :=
+    eapply Permutation_in;
+    [ apply Permutation_map, Permuted_record_sort | ];
+    rewrite map_map;
+    apply_in_map; cbn in *;
+    try lazymatch goal with
+      | H:In (?tag, _, _) ?l |- In ?tag (map ?g ?l) => apply in_map with (f := g) in H
+      end;
+    assumption.
+
+  Ltac prove_is_tbl_ty :=
+    unfold compo_is_tbl_ty; intros;
+    rewrite forallb_forall in *;
+    repeat lazymatch goal with
+      H: forall _, In _ _ -> _, H': In _ _ |- _ =>
+    apply H in H'
+  end; assumption.
+
+  Ltac prove_idx_wf :=
+    unfold aux_wf, aux_wf_for_idx; intros;
+    do 4 (case_match; intuition idtac);
+    unfold compo_idx_wf in *;
+    repeat lazymatch goal with
+    | H:Forall _ ?l, H':In _ ?l |- _ =>
+        let H_new := fresh "H_new" in
+        eapply List.Forall_In in H as H_new; eauto; clear H'
+    end;
+    repeat destruct_match_hyp; intuition idtac;
+    repeat invert_pair; rewrite_l_to_r; try eassumption.
+
+  Lemma mk_idx_sound : forall ic init_tag reps idxs transfs next_tag f,
+      (idxs, transfs, next_tag) = mk_idx init_tag reps ic ->
+      In f transfs ->
+      forall l,
+        incl idxs l ->
+        NoDup (map fst (map fst l)) ->
+        @aug_transf_sound width word ctenv clocals (@IndexInterface.is_tbl_ty (mk_compo_idx l))
+          (@aux_ty (mk_compo_idx l) "id_tag" "aux_tag") (@aux_wf width word (@compo_idx_wf width word l) "id_tag" "aux_tag") f.
+  Proof.
+    destruct ic; cbn; intros; invert_pair; repeat apply_incl_cons_inv.
+    1:{ repeat destruct_In; try apply_in_nil; repeat apply_transf_sound_lemmas.
+        1:{ eapply sum_to_agg_lookup_head_sound; auto using ctenv_ok, clocals_ok.
+            1: prove_aux_ty_for_idx;
+            [ prove_access_record_idx_ty
+            | prove_NoDup_map_fst_sort_map
+            | prove_In_map_fst_sort_map ].
+            1: prove_is_tbl_ty.
+            1: prove_idx_wf. }
+        1:{ apply expr_transf_sound__expr_aug_transf_sound.
+            eapply cons_to_add_head_sound. } }
+    1:{ repeat destruct_In; try apply_in_nil; repeat apply_transf_sound_lemmas.
+        1:{ eapply min_to_agg_lookup_head_sound; auto using ctenv_ok, clocals_ok.
+            1: prove_aux_ty_for_idx;
+            [ prove_access_record_idx_ty
+            | prove_NoDup_map_fst_sort_map
+            | prove_In_map_fst_sort_map ].
+            1: prove_is_tbl_ty.
+            1: prove_idx_wf. }
+        1:{ apply expr_transf_sound__expr_aug_transf_sound.
+            eapply cons_to_min_head_sound. } }
+    1:{ repeat destruct_In; try apply_in_nil; repeat apply_transf_sound_lemmas.
+        1:{ eapply eq_filter_to_lookup_head_sound; auto using ctenv_ok, clocals_ok.
+            1:{ rewrite is_NoDup_to_transparent.
+                instantiate(3:="tup"). instantiate (2:="acc"). instantiate (1:="x").
+                cbn; intuition discriminate. }
+            1: prove_aux_ty_for_idx;
+            [ prove_access_record_idx_ty
+            | prove_NoDup_map_fst_sort_map
+            | prove_In_map_fst_sort_map ].
+            1: prove_is_tbl_ty.
+            1: prove_idx_wf. }
+        1:{ eapply use_idx_head_sound; eauto with transf_hints.
+            1:{ rewrite is_NoDup_to_transparent.
+                instantiate(3:="tup"). instantiate (2:="acc"). instantiate (1:="x").
+                eauto with transf_hints. }
+            1: prove_aux_ty_for_idx;
+            [ prove_access_record_idx_ty
+            | prove_NoDup_map_fst_sort_map
+            | prove_In_map_fst_sort_map ].
+            1: prove_is_tbl_ty.
+            1: prove_idx_wf. }
+        1:{ apply expr_transf_sound__expr_aug_transf_sound.
+            eapply cons_to_insert_head_sound;
+              eauto with transf_hints. } }
+    1:{ repeat destruct_In; try apply_in_nil; repeat apply_transf_sound_lemmas.
+        1:{ eapply filter_to_bitmap_lookup_head_sound;
+              eauto with transf_hints.
+            1:{ rewrite is_NoDup_to_transparent.
+                instantiate(2:="pk_tup"). instantiate (1:="pk_acc").
+                eauto with transf_hints. }
+            1,2: prove_aux_ty_for_idx;
+            [ prove_access_record_idx_ty
+            | prove_NoDup_map_fst_sort_map
+            | prove_In_map_fst_sort_map ].
+            1,2: prove_is_tbl_ty.
+            1,2: prove_idx_wf; instantiate(1:="hole"); auto. }
+        1:{ eapply use_bitmap_head_sound;
+              eauto with transf_hints.
+            1: prove_aux_ty_for_idx;
+            [ prove_access_record_idx_ty
+            | prove_NoDup_map_fst_sort_map
+            | prove_In_map_fst_sort_map ].
+            1: prove_is_tbl_ty.
+            1: prove_idx_wf. }
+        1:{ apply expr_transf_sound__expr_aug_transf_sound.
+            eapply cons_to_bitmap_update_head_sound. }
+        1:{ eapply use_pk_idx_head_sound;
+            eauto with transf_hints.
+            1:{ instantiate(2:="pk_tup"); instantiate(1:="pk_acc");
+                eauto with transf_hints. }
+            1: prove_aux_ty_for_idx;
+            [ prove_access_record_idx_ty
+            | prove_NoDup_map_fst_sort_map
+            | prove_In_map_fst_sort_map ].
+            1: prove_is_tbl_ty.
+            1: prove_idx_wf; instantiate (1:="hole"); assumption. }
+        1:{ apply expr_transf_sound__expr_aug_transf_sound.
+            apply cons_to_pk_idx_update_head_sound. } }
+  Qed.
+
+  Lemma mk_idxs_mk_idx : forall ics init_tag reps idxs transfs next_tag f,
+      (idxs, transfs, next_tag) = mk_idxs init_tag reps ics ->
+      In f transfs ->
+      exists ic init_tag' reps idxs' transfs' next_tag',
+        In ic ics /\
+          (idxs', transfs', next_tag') = mk_idx init_tag' reps ic /\
+          incl idxs' idxs /\
+          In f transfs'.
+  Proof.
+    induction ics; cbn; intros.
+    1:{ invert_pair. apply_in_nil. }
+    1:{ repeat destruct_match_hyp. invert_pair.
+        rewrite in_app_iff in *; intuition idtac.
+        1:{ repeat eexists; eauto using incl_appl, incl_refl. }
+        1:{ eapply IHics in H; eauto.
+            repeat destruct_exists; intuition idtac.
+            repeat eexists; try eassumption;
+              intuition auto using incl_appr. } }
+  Qed.
+
+  Lemma mk_idx_related_transfs_sound : forall ics idxs transfs n init_tag reps,
+      (idxs, transfs, n) = mk_idxs init_tag reps ics ->
+      transf_sound (locals:=clocals) (mk_idx_related_transfs (mk_compo_idx idxs) (mk_idx_use_transfs transfs)).
+  Proof.
+    unfold mk_idx_related_transfs, mk_idx_use_transfs.
+    intros.
+    eapply apply_idx_related_transfs_sound.
+    1: discriminate.
+    apply aug_transf_sound_fold_compose.
+    instantiate (1:=compo_idx_wf idxs).
+    rewrite Forall_forall; intros.
+    eapply mk_idxs_mk_idx in H0; eauto.
+    repeat destruct_exists; intuition idtac.
+    eapply mk_idx_sound; eauto.
+    eapply mk_idxs_ok; eauto.
+    Unshelve.
+    all: eauto with transf_hints.
+    eapply mk_compo_idx_ok; eauto.
+  Qed.
+
+  Theorem apply_all_transfs_sound : forall reps fs icss,
+      transf_sound (locals:=clocals) (apply_all_transfs reps fs icss).
+  Proof.
+    unfold apply_all_transfs; intros.
+    apply transf_sound_compose.
+    2: apply compose_basic_transfs_sound.
+    apply compose_all_idx_transfs_sound.
+    rewrite Forall_forall; intros.
+    rewrite in_map_iff in *.
+    destruct_exists; intuition idtac.
+    repeat destruct_match_hyp. subst.
+    eapply mk_idx_related_transfs_sound; eauto.
+  Qed.
+End WithConcreteMaps.
