conquord/src/conquord/TransfUtils.v
@@ -1,6 +1,6 @@
 Require Import conquord.Language conquord.Interpret conquord.Value conquord.TypeSystem conquord.TypeSound conquord.Utils conquord.TransfSound conquord.IndexInterface.
 Require Import coqutil.Map.Interface coqutil.Word.Interface coqutil.Datatypes.Result.
-Require Import List String ZArith Permutation Morphisms.
+From Stdlib Require Import List String ZArith Permutation Morphisms.
 Import ListNotations.
 
 Ltac apply_type_of__type_wf :=
