README.md
@@ -1,0 +1,5 @@
+A high-level language for data-intensive applications that integrates imperative-language features with query comprehension while enabling formally verified database-style optimizations.
+
+Compiled using the following Rocq version:
+The Rocq Prover, version 9.1.0
+compiled with OCaml 4.14.2
